rocq-osiris/theories/semantics/run.v
@@ -425,26 +425,7 @@ Fixpoint string_of_val (v : val) : string :=
   | VFunctor fields v l  => "VFunctor(Unsupported)"
   | VChar c => "VChar(" ++ string_of_char c ++ ")"
   | VArray l => "VArray(" ++ String.concat "; " (map (fun l => string_of_Z l.(address)) l) ++ ")"
-  | VException e => "VException(" ++ string_of_exception e ++ ")"
   end
-
-with string_of_exception (e : exception) : string :=
-  match e with
-  | Assert_failure => "Assert_failure"
-  | Bad s => "Bad(" ++ s ++ ")"
-  | Continuation_already_resumed => "Continuation_already_resumed"
-  | Division_by_zero => "Division_by_zero"
-  | EmptyStack => "EmptyStack"
-  | EmptyQueue => "EmptyQueue"
-  | Failure s => "Failure(" ++ s ++ ")"
-  | Finally_raised exn => "Finally_raised(" ++ string_of_val exn ++ ")"
-  | Forced_twice => "Forced_twice"
-  | Invalid_argument s => "Invalid_argument"
-  | Match_failure => "Match_failure"
-  | Not_found => "Not_found"
-  | Unhandled eff => "Unhandled"
-  end.
-
 
 Definition string_of_outcome2 (o : outcome2 val exn) : string :=
   match o with
